systems/chord-props/ValidPointersInvariant.v
@@ -94,3 +94,27 @@ Proof using.
     + eapply valid_ptrs_global_net; eauto.
     + eapply valid_ptrs_global_trace; eauto.
 Admitted.
+
+
+Lemma cur_request_valid :
+  forall gst,
+    reachable_st gst ->
+    forall h st dst q m,
+      sigma gst h = Some st ->
+      cur_request st = Some (dst, q, m) ->
+      valid_ptr gst dst.
+Proof.
+  intros.
+  find_apply_lem_hyp valid_ptrs_global_inductive.
+  unfold valid_ptrs_global in *.
+  assert (lift_pred_opt (valid_ptrs_state gst) (Some st)).
+  {
+    repeat find_reverse_rewrite.
+    firstorder.
+  }
+  invcs_prop valid_ptrs_state.
+  unfold valid_ptrs_state, valid_ptrs_cur_request, valid_ptrs_some_cur_request in *.
+  break_and.
+  repeat find_rewrite.
+  inv_prop valid_ptr; tauto.
+Qed.
